Spqr/Specs/Encoding/Polynomial/PolyDecoder/CallMut.lean
@@ -67,6 +67,6 @@ theorem call_mut_spec
       ⦃ (result : (sorted_vec.SortedSet Pt) × PolyDecoder.new_with_poly_count.closure) =>
         result.2 = c ⦄ := by
   unfold call_mut
-  step*
+  simp [sorted_vec.SortedSet.new]
 
 end spqr.encoding.polynomial.PolyDecoder.new_with_poly_count.closure.Insts.CoreOpsFunctionFnMutTupleUsizeSortedSetPt
